riscV/Asm.v
@@ -1277,4 +1277,14 @@ End INSTRSIZE.
 
 (** instrsize instantiation *)
 
-(*** TODO  *)
+Definition instr_size_real (i: instruction) := 32. 
+
+Lemma instr_size_bound_real : forall i, 0 < instr_size_real i <= Ptrofs.max_unsigned.
+Proof.
+  intros. unfold instr_size_real. unfold Ptrofs.max_unsigned.
+  destruct Archi.ptr64 eqn:PTR.
+  rewrite Ptrofs.modulus_eq64;auto. rewrite Int64.modulus_power.
+  unfold Int64.zwordsize. simpl. lia.
+  rewrite Ptrofs.modulus_eq32;auto. rewrite Int.modulus_power.
+  unfold Int.zwordsize. simpl. lia.
+Qed.
