riscV/CompilerAux.v
@@ -1,0 +1,102 @@
+Require Import String.
+Require Import Coqlib Errors.
+Require Import AST Linking Smallstep.
+Require Asm.
+(** RealAsm passed. *)
+(* Require RealAsmgen. *)
+Require PseudoInstructions.
+Require AsmBuiltinInline.
+(* Require AsmStructRet. *)
+(* Require AsmFloatLiteral. *)
+Require AsmLiteral.
+Require AsmPseudoInstr.
+Require Asmlabelgen.
+Require Jumptablegen.
+(** Assembler passes *)
+Require Symbtablegen.
+Require Reloctablesgen.
+Require RelocBingen.
+(* Require AsmLongInt. *)
+(* Require MergeSection. *)
+(* ELF generation *)
+Require RelocElfgen.
+Require EncodeRelocElf.
+
+
+(** * Composing the translation passes *)
+
+(** We first define useful monadic composition operators,
+    along with funny (but convenient) notations. *)
+
+Definition apply_total (A B: Type) (x: res A) (f: A -> B) : res B :=
+  match x with Error msg => Error msg | OK x1 => OK (f x1) end.
+
+Definition apply_partial (A B: Type)
+                         (x: res A) (f: A -> res B) : res B :=
+  match x with Error msg => Error msg | OK x1 => f x1 end.
+
+Notation "a @@@ b" :=
+   (apply_partial _ _ a b) (at level 50, left associativity).
+Notation "a @@ b" :=
+   (apply_total _ _ a b) (at level 50, left associativity).
+
+Definition print {A: Type} (printer: A -> unit) (prog: A) : A :=
+  let unused := printer prog in prog.
+
+Definition time {A B: Type} (name: string) (f: A -> B) : A -> B := f.
+
+Definition total_if {A: Type}
+          (flag: unit -> bool) (f: A -> A) (prog: A) : A :=
+  if flag tt then f prog else prog.
+
+Definition partial_if {A: Type}
+          (flag: unit -> bool) (f: A -> res A) (prog: A) : res A :=
+  if flag tt then f prog else OK prog.
+
+
+Section INSTR_SIZE.
+
+  Variable instr_size : Asm.instruction -> Z.
+  
+  (** TargetPrinter *)
+Definition targetprinter p: res Asm.program :=
+  OK p
+  (* @@ time "SSAsm" SSAsmproof.transf_program *)
+  (* @@@ time "Translation from SSAsm to RealAsm" RealAsmgen.transf_program instr_size *)
+  @@ time "Elimination of pseudo instruction" PseudoInstructions.transf_program
+  @@@ time "Expand builtin inline assembly" AsmBuiltinInline.transf_program
+  (* @@@ time "Pad Instructions with struct return" AsmStructRet.transf_program *)
+  (* @@ time "Generation of the float literal" AsmFloatLiteral.transf_program *)
+  (* @@ time "Generation of int64 literal" AsmLongInt.transf_program (* enable only in 64bit mode?  *) *)
+  @@ time "Generation of the literal" AsmLiteral.transf_program
+  @@ time "Elimination of other pseudo instructions" AsmPseudoInstr.transf_program
+  @@@ time "Make local jumps use offsets instead of labels" Asmlabelgen.transf_program instr_size
+  @@ time "Generation of the jump table" Jumptablegen.transf_program instr_size.
+
+ (* verified part from SACompcert *)
+  (* Definition transf_c_program_real1 p: res Asm.program := *)
+  (* transf_c_program p *)
+  (* @@ time "SSAsm" SSAsmproof.transf_program *)
+  (* @@@ time "Translation from SSAsm to RealAsm" RealAsmgen.transf_program instr_size. *)
+
+ 
+ (** Assembler *)
+ Definition assembler (p: Asm.program) :=
+  OK p
+  @@@ time "Generation of symbol table" Symbtablegen.transf_program instr_size
+  @@@ time "Generation of relocation table" Reloctablesgen.transf_program instr_size
+  @@@ time "Encoding of instructions and data" RelocBingen.transf_program
+  (* @@@ time "Merge Sections" MergeSection.transf_program *)
+  @@@ time "Generation of the reloctable Elf" RelocElfgen.gen_reloc_elf
+  @@@ time "Encoding of the reloctable Elf" EncodeRelocElf.encode_elf_file.
+
+ (* without target printet, used to prove top theorem *)
+ (* Definition transf_c_program_assembler1 (p: Csyntax.program) := *)
+ (*  transf_c_program_real1 p *)
+ (*  @@@ time "Generation of symbol table" Symbtablegen.transf_program instr_size *)
+ (*  @@@ time "Generation of relocation table" Reloctablesgen.transf_program instr_size *)
+ (*  @@@ time "Encoding of instructions and data" RelocBingen.transf_program *)
+ (*  (* @@@ time "Merge Sections" MergeSection.transf_program *) *)
+ (*  @@@ time "Generation of the reloctable Elf" RelocElfgen.gen_reloc_elf *)
+ (*  @@@ time "Encoding of the reloctable Elf" EncodeRelocElf.encode_elf_file. *)
+End INSTR_SIZE.
